books/centaur/fgl/primitives.lisp
@@ -30,230 +30,51 @@
 
 (in-package "FGL")
 
-(include-book "interp-st")
+(include-book "primitives-stub")
 (include-book "bfr-arithmetic")
-(include-book "stack-ev")
-(include-book "scratch-isomorphic")
-(include-book "interp-st-bfrs-ok")
+(include-book "centaur/misc/hons-remove-dups" :dir :system)
+(local (include-book "primitive-lemmas"))
 (local (include-book "centaur/bitops/ihsext-basics" :dir :system))
 (local (std::add-default-post-define-hook :fix))
 
 
-;; BOZO maybe doesn't belong here
-(defsection major-stack-ev-of-interp-st-logicman-extension
 
-  (def-updater-independence-thm gl-object-ev-of-interp-st-logicman-extension
-    (implies (and (logicman-extension-p (interp-st->logicman new) (interp-st->logicman old))
-                  (lbfr-listp (gl-object-bfrlist x) (interp-st->logicman old)))
-             (equal (gl-object-ev x env (interp-st->logicman new))
-                    (gl-object-ev x env (interp-st->logicman old)))))
+     
+(defun gl-primitive-formula-checks (formulas state)
+  (declare (xargs :stobjs state :mode :program))
+  (if (atom formulas)
+      nil
+    (cons `(equal (meta-extract-formula ',(car formulas) state)
+                  ',(meta-extract-formula (car formulas) state))
+          (gl-primitive-formula-checks (cdr formulas) state))))
 
+(defun def-gl-formula-checks-fn (name formulas state)
+  (declare (xargs :stobjs state :mode :program))
+  `(define ,name (state)
+     :returns (ok)
+     (and . ,(gl-primitive-formula-checks formulas state))
+     ///
+     (table gl-formula-checks ',name ',formulas)))
 
-
-  (def-updater-independence-thm gl-objectlist-ev-of-interp-st-logicman-extension
-    (implies (and (logicman-extension-p (interp-st->logicman new) (interp-st->logicman old))
-                  (lbfr-listp (gl-objectlist-bfrlist x) (interp-st->logicman old)))
-             (equal (gl-objectlist-ev x env (interp-st->logicman new))
-                    (gl-objectlist-ev x env (interp-st->logicman old)))))
-
-
-
-  (def-updater-independence-thm gl-object-alist-ev-of-interp-st-logicman-extension
-    (implies (and (logicman-extension-p (interp-st->logicman new) (interp-st->logicman old))
-                  (lbfr-listp (gl-object-alist-bfrlist x) (interp-st->logicman old)))
-             (equal (gl-object-alist-ev x env (interp-st->logicman new))
-                    (gl-object-alist-ev x env (interp-st->logicman old)))))
+(defmacro def-gl-formula-checks (name formulas)
+  `(make-event
+    (def-gl-formula-checks-fn ',name ',formulas state)))
 
 
-
-  (def-updater-independence-thm constraint-instance-of-interp-st-logicman-extension
-    (implies (and (logicman-extension-p (interp-st->logicman new) (interp-st->logicman old))
-                  (lbfr-listp (constraint-instance-bfrlist x) (interp-st->logicman old)))
-             (equal (constraint-instance-ev x env (interp-st->logicman new))
-                    (constraint-instance-ev x env (interp-st->logicman old)))))
-
-
-
-  (def-updater-independence-thm constraint-instancelist-ev-of-interp-st-logicman-extension
-    (implies (and (logicman-extension-p (interp-st->logicman new) (interp-st->logicman old))
-                  (lbfr-listp (constraint-instancelist-bfrlist x) (interp-st->logicman old)))
-             (equal (constraint-instancelist-ev x env (interp-st->logicman new))
-                    (constraint-instancelist-ev x env (interp-st->logicman old)))))
-
-
-
-  (def-updater-independence-thm scratchobj-ev-of-interp-st-logicman-extension
-    (implies (and (logicman-extension-p (interp-st->logicman new) (interp-st->logicman old))
-                  (lbfr-listp (scratchobj->bfrlist x) (interp-st->logicman old)))
-             (equal (scratchobj-ev x env (interp-st->logicman new))
-                    (scratchobj-ev x env (interp-st->logicman old)))))
-
-
-
-  (def-updater-independence-thm scratchlist-ev-of-interp-st-logicman-extension
-    (implies (and (logicman-extension-p (interp-st->logicman new) (interp-st->logicman old))
-                  (lbfr-listp (scratchlist-bfrlist x) (interp-st->logicman old)))
-             (equal (scratchlist-ev x env (interp-st->logicman new))
-                    (scratchlist-ev x env (interp-st->logicman old)))))
-
-
-
-  (def-updater-independence-thm minor-frame-ev-of-interp-st-logicman-extension
-    (implies (and (logicman-extension-p (interp-st->logicman new) (interp-st->logicman old))
-                  (lbfr-listp (minor-frame-bfrlist x) (interp-st->logicman old)))
-             (equal (minor-frame-ev x env (interp-st->logicman new))
-                    (minor-frame-ev x env (interp-st->logicman old)))))
-
-
-
-  (def-updater-independence-thm minor-stack-ev-of-interp-st-logicman-extension
-    (implies (and (logicman-extension-p (interp-st->logicman new) (interp-st->logicman old))
-                  (lbfr-listp (minor-stack-bfrlist x) (interp-st->logicman old)))
-             (equal (minor-stack-ev x env (interp-st->logicman new))
-                    (minor-stack-ev x env (interp-st->logicman old)))))
-
-
-
-  (def-updater-independence-thm major-frame-ev-of-interp-st-logicman-extension
-    (implies (and (logicman-extension-p (interp-st->logicman new) (interp-st->logicman old))
-                  (lbfr-listp (major-frame-bfrlist x) (interp-st->logicman old)))
-             (equal (major-frame-ev x env (interp-st->logicman new))
-                    (major-frame-ev x env (interp-st->logicman old)))))
-
-
-
-  (def-updater-independence-thm major-stack-ev-of-interp-st-logicman-extension
-    (implies (and (logicman-extension-p (interp-st->logicman new) (interp-st->logicman old))
-                  (lbfr-listp (major-stack-bfrlist x) (interp-st->logicman old)))
-             (equal (major-stack-ev x env (interp-st->logicman new))
-                    (major-stack-ev x env (interp-st->logicman old))))))
-
-;; BOZO maybe doesn't belong here
-(define interp-st-scratch-isomorphic (x y)
-  :non-executable t
-  :verify-guards nil
-  (major-stack-scratch-isomorphic (interp-st->stack x) (interp-st->stack y))
-  ///
-  (defequiv interp-st-scratch-isomorphic)
-
-  (defcong interp-st-scratch-isomorphic major-stack-scratch-isomorphic (interp-st->stack x) 1)
-
-  (defcong major-stack-scratch-isomorphic interp-st-scratch-isomorphic (update-interp-st->stack stack x) 1)
-
-  (defthm update-interp-st->stack-norm-under-interp-st-scratch-isomorphic
-    (implies (syntaxp (not (equal x ''nil)))
-             (interp-st-scratch-isomorphic
-              (update-interp-st->stack stack x)
-              (update-interp-st->stack stack nil))))
-
-  (defthm interp-st-scratch-isomorphic-of-update-interp-st->stack-identity
-    (interp-st-scratch-isomorphic
-     (update-interp-st->stack (major-stack-fix (interp-st->stack interp-st)) x)
-     interp-st))
-
-  (defthm interp-st-scratch-isomorphic-of-update-interp-st->stack-identity2
-    (interp-st-scratch-isomorphic
-     (update-interp-st->stack (interp-st->stack interp-st) x)
-     interp-st))
-
-  (def-updater-independence-thm interp-st-scratch-isomorphic-identity
-    (implies (major-stack-equiv (interp-st->stack new) (interp-st->stack old))
-             (equal (interp-st-scratch-isomorphic new x)
-                    (interp-st-scratch-isomorphic old x)))))
-
-(defconst *gl-primitive-thms*
-  '(
-    (defret interp-st-bfrs-ok-of-<fn>
-      (implies (and (interp-st-bfrs-ok interp-st)
-                    (lbfr-listp (gl-objectlist-bfrlist args)
-                                (interp-st->logicman interp-st)))
-               (interp-st-bfrs-ok new-interp-st)))
-
-    (defret bfr-listp-of-<fn>
-      (implies (and
-                (interp-st-bfrs-ok interp-st)
-                (lbfr-listp (gl-objectlist-bfrlist args)
-                            (interp-st->logicman interp-st)))
-               (lbfr-listp (gl-object-bfrlist ans)
-                           (interp-st->logicman new-interp-st))))
-
-    (defret interp-st-get-of-<fn>
-      (implies (and (not (equal (interp-st-field-fix key) :logicman))
-                    (not (equal (interp-st-field-fix key) :stack))
-                    (not (equal (interp-st-field-fix key) :pathcond))
-                    (not (equal (interp-st-field-fix key) :constraint))
-                    (not (equal (interp-st-field-fix key) :bvar-db)))
-               (equal (interp-st-get key new-interp-st)
-                      (interp-st-get key interp-st))))
-
-    (defret major-stack-ev-of-<fn>
-      (equal (major-stack-ev (interp-st->stack new-interp-st) env (interp-st->logicman new-interp-st))
-             (major-stack-ev (interp-st->stack interp-st) env (interp-st->logicman interp-st))))
-
-    (defret scratch-isomorphic-of-<fn>
-      (interp-st-scratch-isomorphic new-interp-st (double-rewrite interp-st)))
-
-    (defret logicman->mode-of-<fn>
-      (equal (logicman->mode (interp-st->logicman new-interp-st))
-             (logicman->mode (interp-st->logicman interp-st))))
-
-    (defret bfr-nvars-of-<fn>
-      (equal (bfr-nvars (interp-st->logicman new-interp-st))
-             (bfr-nvars (interp-st->logicman interp-st))))
-
-    (defret pathcond-enabledp-of-<fn>
-      (iff (nth *pathcond-enabledp* (interp-st->pathcond new-interp-st))
-           (nth *pathcond-enabledp* (interp-st->pathcond interp-st))))
-
-    (defret pathcond-rewind-stack-len-of-<fn>
-      (implies (equal mode (logicman->mode (interp-st->logicman interp-st)))
-               (equal (pathcond-rewind-stack-len mode (interp-st->pathcond new-interp-st))
-                      (pathcond-rewind-stack-len mode (interp-st->pathcond interp-st)))))
-
-    (defret pathcond-rewind-ok-of-<fn>
-      (implies (equal mode (logicman->mode (interp-st->logicman interp-st)))
-               (iff (pathcond-rewind-ok mode (interp-st->pathcond new-interp-st))
-                    (pathcond-rewind-ok mode (interp-st->pathcond interp-st)))))
-
-    (defret pathcond-eval-checkpoints-of-<fn>
-      (equal (logicman-pathcond-eval-checkpoints!
-              env
-              (interp-st->pathcond new-interp-st)
-              (interp-st->logicman new-interp-st))
-             (logicman-pathcond-eval-checkpoints!
-              env
-              (interp-st->pathcond interp-st)
-              (interp-st->logicman interp-st))))
-
-    (defret constraint-eval-of-<fn>
-      (equal (logicman-pathcond-eval
-              env
-              (interp-st->constraint new-interp-st)
-              (interp-st->logicman new-interp-st))
-             (logicman-pathcond-eval
-              env
-              (interp-st->constraint interp-st)
-              (interp-st->logicman interp-st))))
-    
-    (defret get-bvar->term-eval-of-<fn>
-      (iff (fgl-object-eval (get-bvar->term$a n (interp-st->bvar-db new-interp-st))
-                            env
-                            (interp-st->logicman new-interp-st))
-           (fgl-object-eval (get-bvar->term$a n (interp-st->bvar-db interp-st))
-                            env
-                            (interp-st->logicman interp-st))))))
-
-(defun def-gl-primitive-fn (fn formals body)
+(defun def-gl-primitive-fn (fn formals body name-override formula-check-fn prepwork)
   (declare (Xargs :mode :program))
-  (b* ((primfn (intern-in-package-of-symbol
-                (concatenate 'string "GL-" (symbol-name fn) "-PRIMITIVE")
-                'gl-package)))
+  (b* ((primfn (or name-override
+                   (intern-in-package-of-symbol
+                    (concatenate 'string "GL-" (symbol-name fn) "-PRIMITIVE")
+                    'gl-package))))
     `(define ,primfn ((args gl-objectlist-p)
-                      interp-st
+                      (interp-st interp-st-bfrs-ok)
                       state)
+       :guard (interp-st-bfr-listp (gl-objectlist-bfrlist args))
        :returns (mv successp
-                    (ans gl-object-p)
+                    ans
                     new-interp-st)
+       :prepwork ,prepwork
        (if (eql (len args) ,(len formals))
            (b* (((list . ,formals) (gl-objectlist-fix args)))
              ,body)
@@ -262,7 +83,13 @@
        ,@*gl-primitive-thms*
 
        (defret eval-of-<fn>
-         (implies successp
+         (implies (and successp
+                       (fgl-ev-meta-extract-global-facts :state st)
+                       ,@(and formula-check-fn
+                              `((,formula-check-fn st)))
+                       (equal (w st) (w state))
+                       (interp-st-bfrs-ok interp-st)
+                       (interp-st-bfr-listp (gl-objectlist-bfrlist args)))
                   (equal (fgl-object-eval ans env (interp-st->logicman new-interp-st))
                          (fgl-ev (cons ',fn
                                        (kwote-lst (fgl-objectlist-eval args env (interp-st->logicman interp-st))))
@@ -270,121 +97,169 @@
        (table gl-primitives ',fn ',primfn))))
 
 
-(defmacro def-gl-primitive (fn formals body)
-  (def-gl-primitive-fn fn formals body))
+(defmacro def-gl-primitive (fn formals body &key (fnname) (formula-check) (prepwork))
+  (def-gl-primitive-fn fn formals body fnname formula-check prepwork))
+
+
+(defun gl-primitive-fncall-entries (table)
+  (if (atom table)
+      `((otherwise (mv nil nil interp-st)))
+    (b* (((cons fn prim) (car table)))
+      (cons `(,fn (,prim args interp-st state))
+            (gl-primitive-fncall-entries (cdr table))))))
+
+(defun append-alist-vals (x)
+  (if (atom x)
+      nil
+    (append (cdar x)
+            (append-alist-vals (cdr x)))))
+
+(defun formula-check-thms (name table)
+  (if (atom table)
+      nil
+    (b* ((check-name (caar table))
+         (thmname (intern-in-package-of-symbol
+                   (concatenate 'string (symbol-name check-name) "-WHEN-" (symbol-name name))
+                   name)))
+      (cons `(defthm ,thmname
+               (implies (,name st)
+                        (,check-name st))
+               :hints (("Goal" :in-theory '(,name ,check-name))))
+            (formula-check-thms name (cdr table))))))
+
+(set-state-ok t)
+
+(defun install-gl-primitives-fn (name state)
+  (declare (xargs :mode :program))
+  (b* ((wrld (w state))
+       (name-formula-checks (intern-in-package-of-symbol
+                             (concatenate 'string (symbol-name name) "-FORMULA-CHECKS")
+                             name))
+       (formula-checks-table (table-alist 'gl-formula-checks wrld))
+       (all-formulas (gl-primitive-formula-checks
+                      (acl2::hons-remove-dups (append-alist-vals formula-checks-table))
+                      state))
+       (formula-check-thms (formula-check-thms name-formula-checks formula-checks-table)))
+    
+    `(progn
+       (define ,name-formula-checks (state)
+         :ignore-ok t
+         :irrelevant-formals-ok t
+         (and . ,all-formulas)
+         ///
+         . ,formula-check-thms)
+       (define ,name ((fn pseudo-fnsym-p)
+                      (args gl-objectlist-p)
+                      (interp-st interp-st-bfrs-ok)
+                      state)
+         :guard (interp-st-bfr-listp (gl-objectlist-bfrlist args))
+         :returns (mv successp ans new-interp-st)
+         (case (pseudo-fnsym-fix fn)
+           . ,(gl-primitive-fncall-entries (table-alist 'gl-primitives wrld)))
+         ///
+         ,@*gl-primitive-thms*
+         (defret eval-of-<fn>
+           (implies (and successp
+                         (fgl-ev-meta-extract-global-facts :state st)
+                         ;; (,name-formula-checks st)
+                         (equal (w st) (w state))
+                         (interp-st-bfrs-ok interp-st)
+                         (interp-st-bfr-listp (gl-objectlist-bfrlist args)))
+                    (equal (fgl-object-eval ans env (interp-st->logicman new-interp-st))
+                           (fgl-ev (cons (pseudo-fnsym-fix fn)
+                                         (kwote-lst (fgl-objectlist-eval args env (interp-st->logicman interp-st))))
+                                   nil)))))
+
+       ;; bozo, dumb theorem needed to prove fixequiv hook
+       (local (defthm pseudo-fnsym-fix-equal-forward
+                (implies (equal (pseudo-fnsym-fix x) (pseudo-fnsym-fix y))
+                         (pseudo-fnsym-equiv x y))
+                :rule-classes :forward-chaining))
+
+       (defattach
+         (gl-primitive-fncall-stub ,name)
+         ;; (gl-primitive-formula-checks-stub ,name-formula-checks)
+         ))))
+
+(defmacro install-gl-primitives (name)
+  `(make-event
+    (install-gl-primitives-fn ',name state)))
 
 
 (set-ignore-ok t)
 
-(local (defthm fgl-objectlist-eval-when-consp
-         (implies (consp x)
-                  (equal (fgl-objectlist-eval x env)
-                         (cons (fgl-object-eval (car x) env)
-                               (fgl-objectlist-eval (cdr x) env))))
-         :hints(("Goal" :in-theory (enable fgl-objectlist-eval)))))
-
-(local (in-theory (enable gl-objectlist-bfrlist-when-consp)))
-
-(local (defthm len-equal-0
-         (equal (equal (len x) 0)
-                (not (consp x)))))
-
-(local (defthm len-of-cons
-         (equal (len (cons a b))
-                (+ 1 (len b)))))
-
-(local (defun len-is (x n)
-         (if (zp n)
-             (and (eql n 0) (atom x))
-           (and (consp x)
-                (len-is (cdr x) (1- n))))))
-
-(local (defthm open-len-is
-         (implies (syntaxp (quotep n))
-                  (equal (len-is x n)
-                         (if (zp n)
-                             (and (eql n 0) (atom x))
-                           (and (consp x)
-                                (len-is (cdr x) (1- n))))))))
-                         
-
-(local (defthm equal-len-hyp
-         (implies (syntaxp (and (or (acl2::rewriting-negative-literal-fn `(equal (len ,x) ,n) mfc state)
-                                    (acl2::rewriting-negative-literal-fn `(equal ,n (len ,x)) mfc state))
-                                (quotep n)))
-                  (equal (equal (len x) n)
-                         (len-is x n)))))
-
-(local (in-theory (enable* gl-object-bfrlist-when-thms)))
-
-(local (defthm gobj-bfr-list-eval-of-nil
-         (equal (gobj-bfr-list-eval nil x) nil)
-         :hints(("Goal" :in-theory (enable gobj-bfr-list-eval)))))
-
-(local (defthm bools->int-of-single
-         (equal (bools->int (list x))
-                (- (bool->bit x)))
-         :hints(("Goal" :in-theory (enable bools->int)))))
-
-(local (in-theory (disable len)))
-
-(local (defthm bools->int-of-cons
-         (equal (bools->int (cons x y))
-                (if (consp y)
-                    (logcons (bool->bit x) (bools->int y))
-                  (- (bool->bit x))))
-         :hints(("Goal" :in-theory (enable bools->int)))))
-
-(local (defthm logcar-of-bools->int
-         (equal (logcar (bools->int x))
-                (bool->bit (car x)))))
-
-(local (defthm car-of-gobj-bfr-list-eval
-         (equal (car (gobj-bfr-list-eval x env))
-                (gobj-bfr-eval (car x) env))))
-
-(local (defthm scdr-of-gobj-bfr-list-eval
-         (equal (scdr (gobj-bfr-list-eval x env))
-                (gobj-bfr-list-eval (scdr x) env))
-         :hints(("Goal" :in-theory (enable scdr gobj-bfr-list-eval)))))
-
 (def-gl-primitive int (x)
-  (gl-object-case x
-    :g-integer (mv t (gl-object-fix x) interp-st)
-    :otherwise (mv nil nil interp-st)))
+  (b* (((mv ok fix) (gobj-syntactic-integer-fix x))
+       ((unless ok) (mv nil nil interp-st)))
+    (mv t fix interp-st)))
 
 
 (def-gl-primitive endint (x)
   (gl-object-case x
-    :g-boolean (mv t (g-integer (list x.bool)) interp-st)
+    :g-concrete (mv t (if x.val -1 0) interp-st)
+    :g-boolean (mv t (mk-g-integer (list x.bool)) interp-st)
+    :g-cons (mv t -1 interp-st)
+    :g-integer (mv t -1 interp-st)
     :otherwise (mv nil nil interp-st)))
 
+
+
+
 (def-gl-primitive intcons (car cdr)
-  (gl-object-case car
-    :g-boolean (gl-object-case cdr
-                 :g-integer (mv t (g-integer (cons car.bool
-                                                   (if (atom cdr.bits)
-                                                       '(nil)
-                                                     cdr.bits)))
-                                interp-st)
-                 :otherwise (mv nil nil interp-st))
-    :otherwise (mv nil nil interp-st)))
+  (b* (((mv ok car-fix) (gobj-syntactic-boolean-fix car))
+       ((unless ok) (mv nil nil interp-st))
+       ((mv ok cdr-fix) (gobj-syntactic-integer-fix cdr))
+       ((unless ok) (mv nil nil interp-st)))
+    (mv t (mk-g-integer (scons (gobj-syntactic-boolean->bool car-fix)
+                               (gobj-syntactic-integer->bits cdr-fix)))
+        interp-st)))
 
 (table gl-primitives 'intcons* 'gl-intcons-primitive)
 
+(local (defthm logcar-when-not-integerp
+         (implies (not (integerp x))
+                  (equal (logcar x) 0))
+         :hints(("Goal" :in-theory (enable logcar)))))
+
 (def-gl-primitive intcar (x)
   (gl-object-case x
-    :g-integer (mv t (g-boolean (car x.bits)) interp-st)
+    :g-concrete (mv t (and (integerp x.val)
+                           (intcar x.val))
+                    interp-st)
+    :g-integer (mv t (mk-g-boolean (car x.bits)) interp-st)
+    :g-boolean (mv t nil interp-st)
+    :g-cons (mv t nil interp-st)
     :otherwise (mv nil nil interp-st)))
+
+(local (defthm logcdr-when-not-integerp
+         (implies (not (integerp x))
+                  (equal (logcdr x) 0))
+         :hints(("Goal" :in-theory (enable logcdr)))))
+
+(local (in-theory (enable gl-object-kind-when-integerp
+                          g-concrete->val-when-integerp)))
+
+(local (in-theory (disable logcdr-of-bools->int)))
 
 (def-gl-primitive intcdr (x)
   (gl-object-case x
+    :g-concrete (mv t (if (integerp x.val)
+                          (intcdr x.val)
+                        0)
+                    interp-st)
     :g-integer (mv t (g-integer (scdr x.bits)) interp-st)
+    :g-boolean (mv t 0 interp-st)
+    :g-cons (mv t 0 interp-st)
     :otherwise (mv nil nil interp-st)))
+
+(local (in-theory (enable bool-fix)))
 
 (def-gl-primitive bool (x)
   (gl-object-case x
+    :g-concrete (mv t (bool-fix x.val) interp-st)
     :g-boolean (mv t (gl-object-fix x) interp-st)
+    :g-integer (mv t t interp-st)
+    :g-cons (mv t t interp-st)
     :otherwise (mv nil nil interp-st)))
 
 (def-gl-primitive cons (car cdr)
@@ -416,35 +291,122 @@
     :g-cons (mv t x.cdr interp-st)
     :otherwise (mv nil nil interp-st)))
     
-    
+
+(defthm integerp-in-terms-of-int
+  (equal (integerp x)
+         (equal (int x) x))
+  :rule-classes nil)
 
 
-(local
- (defun gl-primitive-fncall-entries (table)
-   (if (atom table)
-       `((otherwise (mv nil nil interp-st)))
-     (b* (((cons fn prim) (car table)))
-       (cons `(,fn (,prim args interp-st state))
-             (gl-primitive-fncall-entries (cdr table)))))))
 
-(make-event
- `(define gl-primitive-fncall ((fn pseudo-fnsym-p)
-                               (args gl-objectlist-p)
-                               (dont)
-                               interp-st
-                               state)
-    :returns (mv successp
-                 (ans gl-object-p)
-                 new-interp-st)
-    (if dont
-        (mv nil nil interp-st)
-      (case (pseudo-fnsym-fix fn)
-        . ,(gl-primitive-fncall-entries (table-alist 'gl-primitives (w state)))))
-    ///
-    ,@*gl-primitive-thms*
-    (defret eval-of-<fn>
-      (implies successp
-               (equal (fgl-object-eval ans env (interp-st->logicman new-interp-st))
-                      (fgl-ev (cons (pseudo-fnsym-fix fn)
-                                    (kwote-lst (fgl-objectlist-eval args env (interp-st->logicman interp-st))))
-                              nil))))))
+
+
+  (local (defthmd gl-object-bfrlist-of-get-bvar->term$a-aux
+           (implies (and (not (member v (bvar-db-bfrlist-aux m bvar-db)))
+                         (< (nfix n) (nfix m))
+                         (<= (base-bvar$a bvar-db) (nfix n)))
+                    (not (member v (gl-object-bfrlist (get-bvar->term$a n bvar-db)))))
+           :hints(("Goal" :in-theory (enable bvar-db-bfrlist-aux)))))
+
+  (local (defthm gl-object-bfrlist-of-get-bvar->term$a
+           (implies (and (not (member v (bvar-db-bfrlist bvar-db)))
+                         (<= (base-bvar$a bvar-db) (nfix n))
+                         (< (nfix n) (next-bvar$a bvar-db)))
+                    (not (member v (gl-object-bfrlist (get-bvar->term$a n bvar-db)))))
+           :hints (("goal" :in-theory (enable bvar-db-bfrlist)
+                    :use ((:instance gl-object-bfrlist-of-get-bvar->term$a-aux
+                           (m (next-bvar$a bvar-db))))))))
+
+;;(local (in-theory (enable gobj-bfr-list-eval-is-bfr-list-eval)))
+
+(define int+ (x y)
+  (+ (ifix x) (ifix y)))
+
+
+
+(def-gl-formula-checks int+-formula-checks (int+ ifix))
+
+(define w-equiv (x y)
+  :non-executable t
+  :no-function t
+  :verify-guards nil
+  (equal (w x) (w y))
+  ///
+  (defequiv w-equiv)
+  (defcong w-equiv equal (w x) 1)
+  (defcong w-equiv equal (meta-extract-formula name state) 2
+    :hints(("Goal" :in-theory (enable meta-extract-formula))))
+
+  (defthm ws-equal-forward
+    (implies (equal (w st) (w state))
+             (w-equiv st state))
+    :rule-classes :forward-chaining))
+
+(local (in-theory (disable w)))
+
+(defthm fgl-ev-of-ifix-call
+  (implies (and (fgl-ev-meta-extract-global-facts :state st)
+                (int+-formula-checks st)
+                (equal (w st) (w state)))
+           (equal (fgl-ev (list 'ifix x) a)
+                  (ifix (fgl-ev x a))))
+  :hints(("Goal" :in-theory (e/d (int+
+                                  int+-formula-checks
+                                  fgl-ev-of-fncall-args)
+                                 (fgl-ev-meta-extract-formula))
+          :use ((:instance fgl-ev-meta-extract-formula
+                 (st state) (state st)
+                 (name 'ifix)
+                 (a (list (cons 'x (fgl-ev x a)))))))))
+
+(defthm fgl-ev-of-int+-call
+  (implies (and (fgl-ev-meta-extract-global-facts :state st)
+                (int+-formula-checks st)
+                (equal (w st) (w state)))
+           (equal (fgl-ev (list 'int+ x y) a)
+                  (int+ (fgl-ev x a)
+                        (fgl-ev y a))))
+  :hints(("Goal" :in-theory (e/d (int+
+                                  int+-formula-checks
+                                  fgl-ev-of-fncall-args)
+                                 (fgl-ev-meta-extract-formula))
+          :use ((:instance fgl-ev-meta-extract-formula
+                 (st state) (state st)
+                 (name 'int+)
+                 (a (list (cons 'x (fgl-ev x a))
+                          (cons 'y (fgl-ev y a)))))))))
+
+(local (defthm fgl-objectlist-eval-of-atom
+         (implies (not (consp x))
+                  (equal (fgl-objectlist-eval x env) nil))
+         :hints(("Goal" :in-theory (enable fgl-objectlist-eval)))
+         :rule-classes ((:rewrite :backchain-limit-lst 0))))
+
+(local (defthm bools->int-of-eval-syntactic-integer-bits
+         (b* (((mv ok xfix) (gobj-syntactic-integer-fix x)))
+           (implies ok
+                    (equal (bools->int (gobj-bfr-list-eval (gobj-syntactic-integer->bits xfix)
+                                                           env))
+                           (ifix (fgl-object-eval x env)))))
+         :hints(("Goal" :in-theory (enable gobj-syntactic-integer->bits
+                                           gobj-syntactic-integer-fix)))))
+
+
+;; (def-gl-primitive int+ (x y)
+;;   (b* (((mv ok xfix) (gobj-syntactic-integer-fix x))
+;;        ((unless ok) (mv nil nil interp-st))
+;;        ((mv ok yfix) (gobj-syntactic-integer-fix y))
+;;        ((unless ok) (mv nil nil interp-st))
+;;        (xbits (gobj-syntactic-integer->bits xfix))
+;;        (ybits (gobj-syntactic-integer->bits yfix)))
+;;     (stobj-let ((logicman (interp-st->logicman interp-st)))
+;;                (bits logicman)
+;;                (bfr-+-ss nil xbits ybits logicman)
+;;                (mv t (mk-g-integer bits) interp-st)))
+;;   :formula-check int+-formula-checks
+;;   :prepwork ((local (in-theory (enable int+)))))
+
+
+
+(install-gl-primitives gl-primitive-fncall-base)
+
