books/centaur/fgl/primitive-lemmas.lisp
@@ -1,0 +1,278 @@
+; GL - A Symbolic Simulation Framework for ACL2
+; Copyright (C) 2019 Centaur Technology
+;
+; Contact:
+;   Centaur Technology Formal Verification Group
+;   7600-C N. Capital of Texas Highway, Suite 300, Austin, TX 78731, USA.
+;   http://www.centtech.com/
+;
+; License: (An MIT/X11-style license)
+;
+;   Permission is hereby granted, free of charge, to any person obtaining a
+;   copy of this software and associated documentation files (the "Software"),
+;   to deal in the Software without restriction, including without limitation
+;   the rights to use, copy, modify, merge, publish, distribute, sublicense,
+;   and/or sell copies of the Software, and to permit persons to whom the
+;   Software is furnished to do so, subject to the following conditions:
+;
+;   The above copyright notice and this permission notice shall be included in
+;   all copies or substantial portions of the Software.
+;
+;   THE SOFTWARE IS PROVIDED "AS IS", WITHOUT WARRANTY OF ANY KIND, EXPRESS OR
+;   IMPLIED, INCLUDING BUT NOT LIMITED TO THE WARRANTIES OF MERCHANTABILITY,
+;   FITNESS FOR A PARTICULAR PURPOSE AND NONINFRINGEMENT. IN NO EVENT SHALL THE
+;   AUTHORS OR COPYRIGHT HOLDERS BE LIABLE FOR ANY CLAIM, DAMAGES OR OTHER
+;   LIABILITY, WHETHER IN AN ACTION OF CONTRACT, TORT OR OTHERWISE, ARISING
+;   FROM, OUT OF OR IN CONNECTION WITH THE SOFTWARE OR THE USE OR OTHER
+;   DEALINGS IN THE SOFTWARE.
+;
+; Original author: Sol Swords <sswords@centtech.com>
+
+(in-package "FGL")
+
+(include-book "logicman")
+(local (include-book "centaur/bitops/ihsext-basics" :dir :system))
+(local (std::add-default-post-define-hook :fix))
+
+(defthm fgl-objectlist-eval-when-consp
+  (implies (consp x)
+           (equal (fgl-objectlist-eval x env)
+                  (cons (fgl-object-eval (car x) env)
+                        (fgl-objectlist-eval (cdr x) env))))
+  :hints(("Goal" :in-theory (enable fgl-objectlist-eval))))
+
+
+(in-theory (enable gl-objectlist-bfrlist-when-consp))
+
+
+
+(in-theory (enable gl-objectlist-bfrlist-when-consp))
+
+(defthm len-equal-0
+  (equal (equal (len x) 0)
+         (not (consp x))))
+
+(defthm len-of-cons
+  (equal (len (cons a b))
+         (+ 1 (len b))))
+
+(defun len-is (x n)
+  (if (zp n)
+      (and (eql n 0) (atom x))
+    (and (consp x)
+         (len-is (cdr x) (1- n)))))
+
+(defthm open-len-is
+  (implies (syntaxp (quotep n))
+           (equal (len-is x n)
+                  (if (zp n)
+                      (and (eql n 0) (atom x))
+                    (and (consp x)
+                         (len-is (cdr x) (1- n)))))))
+                         
+
+(defthm equal-len-hyp
+  (implies (syntaxp (and (or (acl2::rewriting-negative-literal-fn `(equal (len ,x) ,n) mfc state)
+                             (acl2::rewriting-negative-literal-fn `(equal ,n (len ,x)) mfc state))
+                         (quotep n)))
+           (equal (equal (len x) n)
+                  (len-is x n))))
+
+(in-theory (enable* gl-object-bfrlist-when-thms))
+
+(defthm gobj-bfr-list-eval-of-nil
+  (equal (gobj-bfr-list-eval nil x) nil)
+  :hints(("Goal" :in-theory (enable gobj-bfr-list-eval))))
+
+(defthm bools->int-of-single
+  (equal (bools->int (list x))
+         (- (bool->bit x)))
+  :hints(("Goal" :in-theory (enable bools->int))))
+
+(in-theory (disable len))
+
+(defthm bools->int-of-cons
+  (equal (bools->int (cons x y))
+         (if (consp y)
+             (logcons (bool->bit x) (bools->int y))
+           (- (bool->bit x))))
+  :hints(("Goal" :in-theory (enable bools->int))))
+
+(defthm logcar-of-bools->int
+  (equal (logcar (bools->int x))
+         (bool->bit (car x)))
+  :hints(("Goal" :in-theory (enable bools->int))))
+
+(defthm car-of-gobj-bfr-list-eval
+  (equal (car (gobj-bfr-list-eval x env))
+         (gobj-bfr-eval (car x) env)))
+
+(defthm scdr-of-gobj-bfr-list-eval
+  (equal (scdr (gobj-bfr-list-eval x env))
+         (gobj-bfr-list-eval (scdr x) env))
+  :hints(("Goal" :in-theory (enable scdr gobj-bfr-list-eval))))
+
+
+;; BOZO Move all these
+(defthm gl-object-bfrlist-of-mk-g-integer
+  (implies (not (member v bits))
+           (not (member v (gl-object-bfrlist (mk-g-integer bits)))))
+  :hints(("Goal" :in-theory (e/d (mk-g-integer)
+                                 (bools->int)))))
+
+(defthm gl-object-bfrlist-of-mk-g-cons
+  (implies (and (not (member v (gl-object-bfrlist a)))
+                (not (member v (gl-object-bfrlist b))))
+           (not (member v (gl-object-bfrlist (mk-g-cons a b)))))
+  :hints(("Goal" :in-theory (e/d (mk-g-cons)))))
+
+(defthm gl-object-bfrlist-implies-bfr-p-gobj-syntactic-boolean->bool
+  (implies (and (bfr-listp (gl-object-bfrlist x))
+                (gobj-syntactic-booleanp x))
+           (bfr-p (gobj-syntactic-boolean->bool x)))
+  :hints(("Goal" :in-theory (enable gobj-syntactic-booleanp
+                                    gobj-syntactic-boolean->bool
+                                    gl-object-bfrlist
+                                    booleanp))))
+
+(defthm bfr-listp-of-int->bools
+  (bfr-listp (int->bools x))
+  :hints(("Goal" :in-theory (enable int->bools))))
+
+(defthm gl-object-bfrlist-implies-bfr-listp-gobj-syntactic-integer->bits
+  (implies (and (bfr-listp (gl-object-bfrlist x))
+                (gobj-syntactic-integerp x))
+           (bfr-listp (gobj-syntactic-integer->bits x)))
+  :hints(("Goal" :in-theory (enable gobj-syntactic-integerp
+                                    gobj-syntactic-integer->bits
+                                    gl-object-bfrlist))))
+
+
+(defthm bools->int-when-consp
+  (implies (consp b)
+           (equal (bools->int (cons a b))
+                  (intcons a (bools->int b))))
+  :hints(("Goal" :in-theory (enable bools->int))))
+
+(defthm fgl-object-eval-when-gobj-syntactic-booleanp
+  (implies (gobj-syntactic-booleanp x)
+           (equal (fgl-object-eval x env)
+                  (gobj-bfr-eval (gobj-syntactic-boolean->bool x) env)))
+  :hints(("Goal" :in-theory (enable gobj-syntactic-booleanp
+                                    gobj-syntactic-boolean->bool))))
+
+(defret fgl-object-eval-of-gobj-syntactic-boolean-fix
+  (implies okp
+           (equal (gobj-bfr-eval (gobj-syntactic-boolean->bool new-x) env)
+                  (bool-fix (fgl-object-eval x env))))
+  :hints(("Goal" :in-theory (enable gobj-syntactic-boolean->bool
+                                    gobj-syntactic-boolean-fix
+                                    gobj-syntactic-booleanp)))
+  :fn gobj-syntactic-boolean-fix)
+
+(defthm gobj-bfr-list-eval-of-int->bools
+  (equal (gobj-bfr-list-eval (int->bools x) env)
+         (int->bools x))
+  :hints(("Goal" :in-theory (enable int->bools gobj-bfr-list-eval))))
+
+(defthm bools->int-of-int->bools
+  (equal (bools->int (int->bools x))
+         (ifix x))
+  :hints(("Goal" :in-theory (enable int->bools bools->int))))
+
+(defthm fgl-object-eval-when-gobj-syntactic-integerp
+  (implies (gobj-syntactic-integerp x)
+           (equal (fgl-object-eval x env)
+                  (bools->int (gobj-bfr-list-eval (gobj-syntactic-integer->bits x) env))))
+  :hints(("Goal" :in-theory (enable gobj-syntactic-integerp
+                                    gobj-syntactic-integer->bits))))
+
+(defret fgl-object-eval-of-gobj-syntactic-integer-fix
+  (implies okp
+           (equal (bools->int (gobj-bfr-list-eval (gobj-syntactic-integer->bits new-x) env))
+                  (ifix (fgl-object-eval x env))))
+  :hints(("Goal" :in-theory (e/d (gobj-syntactic-integer-fix
+                                  gobj-syntactic-integer->bits
+                                  gl-object-p-when-integerp
+                                  gl-object-kind-when-integerp
+                                  g-concrete->val-when-integerp))))
+  :fn gobj-syntactic-integer-fix)
+
+(defthm gl-object-bfrlist-when-integerp
+  (implies (integerp x)
+           (equal (gl-object-bfrlist x) nil))
+  :hints(("Goal" :in-theory (enable gl-object-kind-when-integerp))))
+
+(defret gl-object-bfrlist-of-gobj-syntactic-integer-fix
+  (implies (not (member v (gl-object-bfrlist x)))
+           (not (member v (gl-object-bfrlist new-x))))
+  :hints(("Goal" :in-theory (enable gobj-syntactic-integer-fix)))
+  :fn gobj-syntactic-integer-fix)
+
+(defret gl-object-bfrlist-of-gobj-syntactic-boolean-fix
+  (implies (not (member v (gl-object-bfrlist x)))
+           (not (member v (gl-object-bfrlist new-x))))
+  :hints(("Goal" :in-theory (enable gobj-syntactic-boolean-fix)))
+  :fn gobj-syntactic-boolean-fix)
+
+
+(Defthm car-of-gl-objectlist-fix
+  (equal (car (gl-objectlist-fix x))
+         (gl-object-fix (car x))))
+
+(in-theory (enable bfr-listp-when-not-member-witness))
+
+
+(defret gobj-bfr-list-eval-of-scons
+  (equal (gobj-bfr-list-eval bits env)
+         (scons (gobj-bfr-eval bit0 env)
+                (gobj-bfr-list-eval rest-bits env)))
+  :hints(("Goal" :in-theory (enable gobj-bfr-list-eval scons)))
+  :fn scons)
+
+
+(defthm equal-of-bfr-listp-witness
+  (implies (bfr-p x bfrstate)
+           (not (equal (bfr-listp-witness lst bfrstate) x))))
+
+
+
+
+(defthm gl-object-bfrlist-when-booleanp
+  (implies (booleanp x)
+           (equal (gl-object-bfrlist x) nil))
+  :hints(("Goal" :in-theory (enable gl-object-bfrlist
+                                    gl-object-kind))))
+
+
+
+(defthm gobj-syntactic-listp-when-gobj-syntactic-consp
+  (implies (gobj-syntactic-consp x)
+           (gobj-syntactic-listp x))
+  :hints(("Goal" :in-theory (enable gobj-syntactic-listp
+                                    gobj-syntactic-consp))))
+
+(defthm gl-object-bfrlist-of-gobj-syntactic-list->car
+  (implies (not (member v (gl-object-bfrlist x)))
+           (not (member v (gl-object-bfrlist (gobj-syntactic-list->car x)))))
+  :hints(("Goal" :in-theory (enable gobj-syntactic-list->car))))
+
+(defthm gl-object-bfrlist-of-gobj-syntactic-list->cdr
+  (implies (not (member v (gl-object-bfrlist x)))
+           (not (member v (gl-object-bfrlist (gobj-syntactic-list->cdr x)))))
+  :hints(("Goal" :in-theory (enable gobj-syntactic-list->cdr))))
+
+(defthm fgl-object-eval-of-mk-g-cons
+  (equal (fgl-object-eval (mk-g-cons a b) env)
+         (cons (fgl-object-eval a env)
+               (fgl-object-eval b env)))
+  :hints(("Goal" :in-theory (enable mk-g-cons))))
+
+(defthmd fgl-object-eval-when-gobj-syntactic-consp
+  (implies (gobj-syntactic-consp x)
+           (equal (fgl-object-eval x env)
+                  (cons (fgl-object-eval (gobj-syntactic-list->car x) env)
+                        (fgl-object-eval (gobj-syntactic-list->cdr x) env))))
+  :hints(("Goal" :in-theory (enable gobj-syntactic-consp
+                                    gobj-syntactic-list->cdr
+                                    gobj-syntactic-list->car))))
