books/centaur/fgl/primitives-stub.lisp
@@ -1,0 +1,341 @@
+; GL - A Symbolic Simulation Framework for ACL2
+; Copyright (C) 2019 Centaur Technology
+;
+; Contact:
+;   Centaur Technology Formal Verification Group
+;   7600-C N. Capital of Texas Highway, Suite 300, Austin, TX 78731, USA.
+;   http://www.centtech.com/
+;
+; License: (An MIT/X11-style license)
+;
+;   Permission is hereby granted, free of charge, to any person obtaining a
+;   copy of this software and associated documentation files (the "Software"),
+;   to deal in the Software without restriction, including without limitation
+;   the rights to use, copy, modify, merge, publish, distribute, sublicense,
+;   and/or sell copies of the Software, and to permit persons to whom the
+;   Software is furnished to do so, subject to the following conditions:
+;
+;   The above copyright notice and this permission notice shall be included in
+;   all copies or substantial portions of the Software.
+;
+;   THE SOFTWARE IS PROVIDED "AS IS", WITHOUT WARRANTY OF ANY KIND, EXPRESS OR
+;   IMPLIED, INCLUDING BUT NOT LIMITED TO THE WARRANTIES OF MERCHANTABILITY,
+;   FITNESS FOR A PARTICULAR PURPOSE AND NONINFRINGEMENT. IN NO EVENT SHALL THE
+;   AUTHORS OR COPYRIGHT HOLDERS BE LIABLE FOR ANY CLAIM, DAMAGES OR OTHER
+;   LIABILITY, WHETHER IN AN ACTION OF CONTRACT, TORT OR OTHERWISE, ARISING
+;   FROM, OUT OF OR IN CONNECTION WITH THE SOFTWARE OR THE USE OR OTHER
+;   DEALINGS IN THE SOFTWARE.
+;
+; Original author: Sol Swords <sswords@centtech.com>
+
+(in-package "FGL")
+
+(include-book "interp-st")
+(include-book "stack-ev")
+(include-book "scratch-isomorphic")
+(include-book "interp-st-bfrs-ok")
+(local (std::add-default-post-define-hook :fix))
+
+
+(acl2::def-meta-extract fgl-ev fgl-ev-list)
+
+;; BOZO maybe doesn't belong here
+(defsection major-stack-ev-of-interp-st-logicman-extension
+
+  (def-updater-independence-thm gl-object-ev-of-interp-st-logicman-extension
+    (implies (and (logicman-extension-p (interp-st->logicman new) (interp-st->logicman old))
+                  (lbfr-listp (gl-object-bfrlist x) (interp-st->logicman old)))
+             (equal (gl-object-ev x env (interp-st->logicman new))
+                    (gl-object-ev x env (interp-st->logicman old)))))
+
+
+
+  (def-updater-independence-thm gl-objectlist-ev-of-interp-st-logicman-extension
+    (implies (and (logicman-extension-p (interp-st->logicman new) (interp-st->logicman old))
+                  (lbfr-listp (gl-objectlist-bfrlist x) (interp-st->logicman old)))
+             (equal (gl-objectlist-ev x env (interp-st->logicman new))
+                    (gl-objectlist-ev x env (interp-st->logicman old)))))
+
+
+
+  (def-updater-independence-thm gl-object-alist-ev-of-interp-st-logicman-extension
+    (implies (and (logicman-extension-p (interp-st->logicman new) (interp-st->logicman old))
+                  (lbfr-listp (gl-object-alist-bfrlist x) (interp-st->logicman old)))
+             (equal (gl-object-alist-ev x env (interp-st->logicman new))
+                    (gl-object-alist-ev x env (interp-st->logicman old)))))
+
+
+
+  (def-updater-independence-thm constraint-instance-of-interp-st-logicman-extension
+    (implies (and (logicman-extension-p (interp-st->logicman new) (interp-st->logicman old))
+                  (lbfr-listp (constraint-instance-bfrlist x) (interp-st->logicman old)))
+             (equal (constraint-instance-ev x env (interp-st->logicman new))
+                    (constraint-instance-ev x env (interp-st->logicman old)))))
+
+
+
+  (def-updater-independence-thm constraint-instancelist-ev-of-interp-st-logicman-extension
+    (implies (and (logicman-extension-p (interp-st->logicman new) (interp-st->logicman old))
+                  (lbfr-listp (constraint-instancelist-bfrlist x) (interp-st->logicman old)))
+             (equal (constraint-instancelist-ev x env (interp-st->logicman new))
+                    (constraint-instancelist-ev x env (interp-st->logicman old)))))
+
+
+
+  (def-updater-independence-thm scratchobj-ev-of-interp-st-logicman-extension
+    (implies (and (logicman-extension-p (interp-st->logicman new) (interp-st->logicman old))
+                  (lbfr-listp (scratchobj->bfrlist x) (interp-st->logicman old)))
+             (equal (scratchobj-ev x env (interp-st->logicman new))
+                    (scratchobj-ev x env (interp-st->logicman old)))))
+
+
+
+  (def-updater-independence-thm scratchlist-ev-of-interp-st-logicman-extension
+    (implies (and (logicman-extension-p (interp-st->logicman new) (interp-st->logicman old))
+                  (lbfr-listp (scratchlist-bfrlist x) (interp-st->logicman old)))
+             (equal (scratchlist-ev x env (interp-st->logicman new))
+                    (scratchlist-ev x env (interp-st->logicman old)))))
+
+
+
+  (def-updater-independence-thm minor-frame-ev-of-interp-st-logicman-extension
+    (implies (and (logicman-extension-p (interp-st->logicman new) (interp-st->logicman old))
+                  (lbfr-listp (minor-frame-bfrlist x) (interp-st->logicman old)))
+             (equal (minor-frame-ev x env (interp-st->logicman new))
+                    (minor-frame-ev x env (interp-st->logicman old)))))
+
+
+
+  (def-updater-independence-thm minor-stack-ev-of-interp-st-logicman-extension
+    (implies (and (logicman-extension-p (interp-st->logicman new) (interp-st->logicman old))
+                  (lbfr-listp (minor-stack-bfrlist x) (interp-st->logicman old)))
+             (equal (minor-stack-ev x env (interp-st->logicman new))
+                    (minor-stack-ev x env (interp-st->logicman old)))))
+
+
+
+  (def-updater-independence-thm major-frame-ev-of-interp-st-logicman-extension
+    (implies (and (logicman-extension-p (interp-st->logicman new) (interp-st->logicman old))
+                  (lbfr-listp (major-frame-bfrlist x) (interp-st->logicman old)))
+             (equal (major-frame-ev x env (interp-st->logicman new))
+                    (major-frame-ev x env (interp-st->logicman old)))))
+
+
+
+  (def-updater-independence-thm major-stack-ev-of-interp-st-logicman-extension
+    (implies (and (logicman-extension-p (interp-st->logicman new) (interp-st->logicman old))
+                  (lbfr-listp (major-stack-bfrlist x) (interp-st->logicman old)))
+             (equal (major-stack-ev x env (interp-st->logicman new))
+                    (major-stack-ev x env (interp-st->logicman old))))))
+
+;; BOZO maybe doesn't belong here
+(define interp-st-scratch-isomorphic (x y)
+  :non-executable t
+  :verify-guards nil
+  (major-stack-scratch-isomorphic (interp-st->stack x) (interp-st->stack y))
+  ///
+  (defequiv interp-st-scratch-isomorphic)
+
+  (defcong interp-st-scratch-isomorphic major-stack-scratch-isomorphic (interp-st->stack x) 1)
+
+  (defcong major-stack-scratch-isomorphic interp-st-scratch-isomorphic (update-interp-st->stack stack x) 1)
+
+  (defthm update-interp-st->stack-norm-under-interp-st-scratch-isomorphic
+    (implies (syntaxp (not (equal x ''nil)))
+             (interp-st-scratch-isomorphic
+              (update-interp-st->stack stack x)
+              (update-interp-st->stack stack nil))))
+
+  (defthm interp-st-scratch-isomorphic-of-update-interp-st->stack-identity
+    (interp-st-scratch-isomorphic
+     (update-interp-st->stack (major-stack-fix (interp-st->stack interp-st)) x)
+     interp-st))
+
+  (defthm interp-st-scratch-isomorphic-of-update-interp-st->stack-identity2
+    (interp-st-scratch-isomorphic
+     (update-interp-st->stack (interp-st->stack interp-st) x)
+     interp-st))
+
+  (def-updater-independence-thm interp-st-scratch-isomorphic-identity
+    (implies (major-stack-equiv (interp-st->stack new) (interp-st->stack old))
+             (equal (interp-st-scratch-isomorphic new x)
+                    (interp-st-scratch-isomorphic old x)))))
+
+(defconst *gl-primitive-thms*
+  '(
+    (defret gl-object-p-ans-of-<fn>
+      (gl-object-p ans))
+    
+    (defret interp-st-bfrs-ok-of-<fn>
+      (implies (and (interp-st-bfrs-ok interp-st)
+                    (lbfr-listp (gl-objectlist-bfrlist args)
+                                (interp-st->logicman interp-st)))
+               (interp-st-bfrs-ok new-interp-st)))
+
+    (defret bfr-listp-of-<fn>
+      (implies (and
+                (interp-st-bfrs-ok interp-st)
+                (lbfr-listp (gl-objectlist-bfrlist args)
+                            (interp-st->logicman interp-st)))
+               (lbfr-listp (gl-object-bfrlist ans)
+                           (interp-st->logicman new-interp-st))))
+
+    (defret interp-st-get-of-<fn>
+      (implies (and (not (equal (interp-st-field-fix key) :logicman))
+                    (not (equal (interp-st-field-fix key) :stack))
+                    (not (equal (interp-st-field-fix key) :pathcond))
+                    (not (equal (interp-st-field-fix key) :constraint))
+                    (not (equal (interp-st-field-fix key) :bvar-db)))
+               (equal (interp-st-get key new-interp-st)
+                      (interp-st-get key interp-st))))
+
+    (defret major-stack-ev-of-<fn>
+      (implies (interp-st-bfrs-ok interp-st)
+               (equal (major-stack-ev (interp-st->stack new-interp-st) env (interp-st->logicman new-interp-st))
+                      (major-stack-ev (interp-st->stack interp-st) env (interp-st->logicman interp-st)))))
+
+    (defret scratch-isomorphic-of-<fn>
+      (interp-st-scratch-isomorphic new-interp-st (double-rewrite interp-st)))
+
+    (defret logicman->mode-of-<fn>
+      (equal (logicman->mode (interp-st->logicman new-interp-st))
+             (logicman->mode (interp-st->logicman interp-st))))
+
+    (defret bfr-nvars-of-<fn>
+      (equal (bfr-nvars (interp-st->logicman new-interp-st))
+             (bfr-nvars (interp-st->logicman interp-st))))
+
+    (defret pathcond-enabledp-of-<fn>
+      (iff (nth *pathcond-enabledp* (interp-st->pathcond new-interp-st))
+           (nth *pathcond-enabledp* (interp-st->pathcond interp-st))))
+
+    (defret pathcond-rewind-stack-len-of-<fn>
+      (implies (equal mode (logicman->mode (interp-st->logicman interp-st)))
+               (equal (pathcond-rewind-stack-len mode (interp-st->pathcond new-interp-st))
+                      (pathcond-rewind-stack-len mode (interp-st->pathcond interp-st)))))
+
+    (defret pathcond-rewind-ok-of-<fn>
+      (implies (equal mode (logicman->mode (interp-st->logicman interp-st)))
+               (iff (pathcond-rewind-ok mode (interp-st->pathcond new-interp-st))
+                    (pathcond-rewind-ok mode (interp-st->pathcond interp-st)))))
+
+    (defret pathcond-eval-checkpoints-of-<fn>
+      (implies (interp-st-bfrs-ok interp-st)
+               (equal (logicman-pathcond-eval-checkpoints!
+                       env
+                       (interp-st->pathcond new-interp-st)
+                       (interp-st->logicman new-interp-st))
+                      (logicman-pathcond-eval-checkpoints!
+                       env
+                       (interp-st->pathcond interp-st)
+                       (interp-st->logicman interp-st)))))
+
+    (defret constraint-eval-of-<fn>
+      (implies (interp-st-bfrs-ok interp-st)
+               (equal (logicman-pathcond-eval
+                       env
+                       (interp-st->constraint new-interp-st)
+                       (interp-st->logicman new-interp-st))
+                      (logicman-pathcond-eval
+                       env
+                       (interp-st->constraint interp-st)
+                       (interp-st->logicman interp-st)))))
+    
+    (defret get-bvar->term-eval-of-<fn>
+      (b* ((bvar-db (interp-st->bvar-db interp-st)))
+        (implies (and (interp-st-bfrs-ok interp-st)
+                      (<= (base-bvar$a bvar-db) (nfix n))
+                      (< (nfix n) (next-bvar$a bvar-db)))
+                 (iff (fgl-object-eval (get-bvar->term$a n (interp-st->bvar-db new-interp-st))
+                                       env
+                                       (interp-st->logicman new-interp-st))
+                      (fgl-object-eval (get-bvar->term$a n bvar-db)
+                                       env
+                                       (interp-st->logicman interp-st))))))
+
+    (defret next-bvar-of-<fn>
+      (equal (next-bvar$a (interp-st->bvar-db new-interp-st))
+             (next-bvar$a (interp-st->bvar-db interp-st))))
+
+    (defret base-bvar-of-<fn>
+      (equal (base-bvar$a (interp-st->bvar-db new-interp-st))
+             (base-bvar$a (interp-st->bvar-db interp-st))))))
+
+
+
+(make-event 
+ `(encapsulate
+    (((gl-primitive-fncall-stub * * interp-st state) => (mv * * interp-st)
+      :formals (fn args interp-st state)
+      :guard (and (pseudo-fnsym-p fn)
+                  (gl-objectlist-p args)
+                  (interp-st-bfrs-ok interp-st)
+                  (interp-st-bfr-listp (gl-objectlist-bfrlist args))))
+     ;; ((gl-primitive-formula-checks-stub state) => *
+     ;;  :formals (state))
+     )
+                                              
+
+    ;; (local (define gl-primitive-formula-checks-stub (state)
+    ;;          :ignore-ok t
+    ;;          :irrelevant-formals-ok t
+    ;;          :returns (okp)
+    ;;          t))
+
+
+    (local (define gl-primitive-fncall-stub ((fn pseudo-fnsym-p)
+                                             (args gl-objectlist-p)
+                                             (interp-st interp-st-bfrs-ok)
+                                             state)
+             :guard (interp-st-bfr-listp (gl-objectlist-bfrlist args))
+             :ignore-ok t
+             :irrelevant-formals-ok t
+             :returns (mv successp ans new-interp-st)
+             (mv nil nil interp-st)))
+
+    (local (in-theory (enable gl-primitive-fncall-stub)))
+
+    ,@*gl-primitive-thms*
+
+    (defret eval-of-<fn>
+      (implies (and successp
+                    (fgl-ev-meta-extract-global-facts :state st)
+                    ;; (gl-primitive-formula-checks-stub st)
+                    (equal (w st) (w state))
+                    (interp-st-bfrs-ok interp-st)
+                    (interp-st-bfr-listp (gl-objectlist-bfrlist args)))
+               (equal (fgl-object-eval ans env (interp-st->logicman new-interp-st))
+                      (fgl-ev (cons (pseudo-fnsym-fix fn)
+                                    (kwote-lst (fgl-objectlist-eval args env (interp-st->logicman interp-st))))
+                              nil))))
+
+    (deffixequiv gl-primitive-fncall-stub)))
+
+
+
+(make-event
+ `(define gl-primitive-fncall ((fn pseudo-fnsym-p)
+                               (args gl-objectlist-p)
+                               (dont)
+                               (interp-st interp-st-bfrs-ok) 
+                               state)
+    :guard (interp-st-bfr-listp (gl-objectlist-bfrlist args))
+    :returns (mv successp
+                 (ans gl-object-p)
+                 new-interp-st)
+    (if dont
+        (mv nil nil interp-st)
+      (gl-primitive-fncall-stub fn args interp-st state))
+    ///
+    ,@*gl-primitive-thms*
+    (defret eval-of-<fn>
+      (implies (and successp
+                    (fgl-ev-meta-extract-global-facts :state st)
+                    ;; (gl-primitive-formula-checks-stub st)
+                    (equal (w st) (w state))
+                    (interp-st-bfrs-ok interp-st)
+                    (interp-st-bfr-listp (gl-objectlist-bfrlist args)))
+               (equal (fgl-object-eval ans env (interp-st->logicman new-interp-st))
+                      (fgl-ev (cons (pseudo-fnsym-fix fn)
+                                    (kwote-lst (fgl-objectlist-eval args env (interp-st->logicman interp-st))))
+                              nil))))))
